porting to autosubst complete

theories/DeclarativeTyping.v
@@ -186,13 +186,12 @@ Definition WfDeclInductionConcl
 	× (forall (Γ : context) (A B : term), [Γ |- A ≅ B] -> PTyEq Γ A B)
   × (forall (Γ : context) (A t u : term), [Γ |- t ≅ u : A] -> PTmEq Γ A t u).
 
-Let WfDeclInductionType := ltac:
-  (
-  set (H := _WfDeclInduction) ;
-  fold_decl ;
-  let ty := type of H in exact ty).
-
-Definition WfDeclInduction : WfDeclInductionType := _WfDeclInduction.
+Definition WfDeclInduction :=
+  ltac:(let ind := fresh "ind" in
+      pose (ind := _WfDeclInduction);
+      fold_decl ;
+      let ind_ty := type of ind in
+      exact (ind : ind_ty)).
 
 End InductionPrinciples.
 
@@ -248,7 +247,7 @@ Section TypingWk.
 
   Theorem typing_wk : WfDeclInductionConcl PCon PTy PTm PTyEq PTmEq.
   Proof.
-    apply WfDeclInduction.
+    apply _WfDeclInduction.
     - red.
       trivial.
     - red. trivial.
@@ -398,3 +397,84 @@ Section TypingWk.
   Qed.
 
 End TypingWk.
+
+Section WfContext.
+  Import DeclarativeTypingData.
+
+  Definition concons_inv {Γ na A} : [|- Γ,, vass na A] -> [|- Γ].
+  Proof.
+    now inversion 1.
+  Qed.
+
+  Definition concons_inv' {Γ na A} : [|- Γ,, vass na A] -> [Γ |- A].
+  Proof.
+    now inversion 1.
+  Qed.
+
+  Definition WFterm {Γ} {t A} :
+      [ Γ |- t : A ] -> 
+      [ |- Γ ].
+  Proof.
+    induction 1 ; tea.
+    now eapply concons_inv.
+  Qed.
+
+  Definition WFtype {Γ} {A} :
+      [ Γ |- A ] -> 
+      [ |- Γ ].
+  Proof.
+      induction 1; tea.
+      now eapply WFterm.
+  Qed.
+
+
+  Definition WFEqTerm {Γ} {t u A} :
+      [ Γ |- t ≅ u : A ] -> 
+      [ |- Γ ].
+  Proof.
+      induction 1 ; eauto.
+      all: eapply WFterm ; eassumption.
+  Qed.
+
+  Definition WFEqType {Γ} {A B} :
+      [ Γ |- A ≅ B ] -> 
+      [ |- Γ ].
+  Proof.
+    induction 1 ; eauto.
+    1: now eapply WFtype.
+    now eapply WFEqTerm.
+  Qed.
+
+  Definition redFirstTerm {Γ t u A} : 
+    [ Γ |- t ⇒ u : A] ->
+    [ Γ |- t : A ].
+  Proof.
+    induction 1.
+    all: econstructor ; eauto.
+    now econstructor.
+  Qed.
+
+  Definition redFirst {Γ A B} : 
+    [ Γ |- A ⇒ B ] ->
+    [ Γ |- A ].
+  Proof.
+    destruct 1.
+    econstructor.
+    now eapply redFirstTerm.
+  Qed.
+
+  Definition redFirstCTerm {Γ t u A} : 
+    [ Γ |- t ⇒* u : A] ->
+    [ Γ |- t : A ].
+  Proof.
+    induction 1 ; eauto using redFirstTerm.
+  Qed.
+
+  Definition redFirstC {Γ A B} : 
+    [ Γ |- A ⇒* B ] ->
+    [ Γ |- A ].
+  Proof.
+    induction 1 ; eauto using redFirst.
+  Qed.
+
+End WfContext.
