theories/Utils.v
@@ -1,4 +1,4 @@
-From Coq Require Import Morphisms List.
+From Coq Require Import Morphisms List CRelationClasses.
 From MetaCoq Require Export MCPrelude MCProd.
 From LogRel.AutoSubst Require Import core.
 
@@ -7,6 +7,7 @@ Notation "`=1`" := (pointwise_relation _ Logic.eq) (at level 80).
 Infix "=1" := (pointwise_relation _ Logic.eq) (at level 70).
 Notation "`=2`" := (pointwise_relation _ (pointwise_relation _ Logic.eq)) (at level 80).
 Infix "=2" := (pointwise_relation _ (pointwise_relation _ Logic.eq)) (at level 70).
+Infix "<~>" := iffT (at level 90).
 
 (* The database used for generic typing *)
 Create HintDb gen_typing.
